x64 invariants: CSpace_AI checking
Includes some changes to the abstract spec:
- replace magic numbers with definitions.
- add missing IOPortCap cases to some definitions.

There is one sorry proof, which I think blast could solve if we
gave it enough time. Will need a more subtle approach.

spec/abstract/X64/Arch_Structs_A.thy
@@ -41,9 +41,9 @@ along with capabilities for IO ports and spaces, as well as virtual memory mappi
 datatype vm_map_type = VMNoMap | VMVSpaceMap | VMIOSpaceMap
 
 datatype arch_cap =
-   ASIDPoolCap (cap_asid_pool : obj_ref) (cap_asid_base : asid)
+   ASIDPoolCap (acap_asid_pool : obj_ref) (acap_asid_base : asid)
  | ASIDControlCap
- | IOPortCap (cap_io_port_first_port : io_port) (cap_io_port_last_port : io_port)
+ | IOPortCap (acap_io_port_first_port : io_port) (acap_io_port_last_port : io_port)
 (* FIXME x64-vtd:
  | IOSpaceCap (cap_io_domain_id : "16 word") (cap_io_pci_device : "io_asid option")
  | IOPageTableCap (cap_iopt_base_ptr : obj_ref) (cap_io_pt_level : nat) (cap_iopt_mapped_address : "(io_asid * vspace_ref) option")
