proof/invariant-abstract/BCorres_AI.thy
@@ -204,7 +204,7 @@ lemma throw_on_false_bcorres[wp]: "bcorres f f' \<Longrightarrow>  bcorres (thro
   done
 
 context Arch begin
-  crunch (bcorres)bcorres[wp]: arch_finalise_cap truncate_state (simp: swp_def)
+  crunch (bcorres)bcorres[wp]: arch_finalise_cap truncate_state (simp: swp_def ignore: forM_x)
 end
 
 requalify_facts Arch.arch_finalise_cap_bcorres
