proof/invariant-abstract/X64/ArchCSpacePre_AI.thy
@@ -29,14 +29,19 @@ definition
      (case ac of
          ASIDPoolCap r as \<Rightarrow> True
        | ASIDControlCap \<Rightarrow> False
-       | PageCap r rghts sz mapdata \<Rightarrow> False
+       | IOPortCap first_port last_port \<Rightarrow> True (* FIXME: stab in the dark. *)
+       | PageCap r rghts maptype sz mapdata \<Rightarrow> False
        | PageTableCap r mapdata \<Rightarrow> True
-       | PageDirectoryCap r mapdata \<Rightarrow> True)"
+       | PageDirectoryCap r mapdata \<Rightarrow> True
+       | PDPointerTableCap r mapdata \<Rightarrow> True
+       | PML4Cap r mapdata \<Rightarrow> True)"
 
 definition
-  "cap_vptr_arch acap \<equiv> case acap of 
-     (PageCap _ _ _ (Some (_, vptr))) \<Rightarrow> Some vptr
+  "cap_vptr_arch acap \<equiv> case acap of
+     (PageCap _ _ _ _ (Some (_, vptr))) \<Rightarrow> Some vptr
   |  (PageTableCap _ (Some (_, vptr))) \<Rightarrow> Some vptr
+  |  (PageDirectoryCap _ (Some (_, vptr))) \<Rightarrow> Some vptr
+  |  (PDPointerTableCap _ (Some (_, vptr))) \<Rightarrow> Some vptr
   | _ \<Rightarrow> None"
 
 definition
@@ -47,52 +52,48 @@ declare cap_vptr_arch_def[abs_def, simp]
 lemmas cap_vptr_simps [simp] = 
   cap_vptr_def [simplified, split_simps cap.split arch_cap.split option.split prod.split]
 
+(* True when cap' is derived from cap. *)
 definition
-  "is_derived_arch cap cap' \<equiv>
-    ((is_pt_cap cap \<or> is_pd_cap cap) \<longrightarrow> 
-         cap_asid cap = cap_asid cap' \<and> cap_asid cap \<noteq> None) \<and>
-     (vs_cap_ref cap = vs_cap_ref cap' \<or> is_pg_cap cap')"
+  "is_derived_arch cap' cap \<equiv>
+    (is_vspace_table_cap cap' \<longrightarrow> cap_asid cap = cap_asid cap' \<and> cap_asid cap' \<noteq> None) \<and>
+    (vs_cap_ref cap = vs_cap_ref cap' \<or> is_pg_cap cap)"
 
 lemma is_derived_arch_non_arch:
-  "\<not>is_arch_cap cap \<Longrightarrow> \<not> is_arch_cap cap' \<Longrightarrow> 
-      is_derived_arch cap cap'"
-  unfolding is_derived_arch_def is_pg_cap_def is_pt_cap_def is_pd_cap_def
-            vs_cap_ref_def is_arch_cap_def
+  "\<not> is_arch_cap cap \<Longrightarrow> \<not> is_arch_cap cap' \<Longrightarrow> is_derived_arch cap cap'"
+  unfolding is_derived_arch_def vs_cap_ref_def is_arch_cap_def
+            is_pg_cap_def is_pt_cap_def is_pd_cap_def is_pdpt_cap_def is_pml4_cap_def
   by (auto split: cap.splits)
 
 lemma is_derived_cap_arch_asid:
-  "is_derived_arch cap cap' \<Longrightarrow> cap_master_cap cap = cap_master_cap cap' \<Longrightarrow> 
-      is_pt_cap cap' \<or> is_pd_cap cap' \<Longrightarrow> cap_asid cap = cap_asid cap'"
+  "is_derived_arch cap cap' \<Longrightarrow> cap_master_cap cap = cap_master_cap cap'
+    \<Longrightarrow> is_vspace_table_cap cap' \<Longrightarrow> cap_asid cap = cap_asid cap'"
   unfolding is_derived_arch_def
   apply (cases cap; cases cap'; simp)
   by (auto simp: is_cap_simps cap_master_cap_def split: arch_cap.splits)
 
-
 lemma is_page_cap_PageCap[simp]:
-  "is_page_cap (PageCap ref rghts pgsiz mapdata)"
+  "is_page_cap (PageCap ref rghts maptype pgsiz mapdata)"
   by (simp add: is_page_cap_def)
 
 lemma pageBitsForSize_eq[simp]:
   "(pageBitsForSize sz = pageBitsForSize sz') = (sz = sz')"
-by (case_tac sz) (case_tac sz', simp+)+
+  by (cases sz; cases sz'; simp add: pageBits_def ptTranslationBits_def)
 
 
 lemma
   cap_master_cap_arch_simps:
-  "cap_master_arch_cap ((arch_cap.PageCap ref rghts sz mapdata)) =
-         (arch_cap.PageCap ref UNIV sz None)"
-  "cap_master_arch_cap ( (arch_cap.ASIDPoolCap pool asid)) =
-          (arch_cap.ASIDPoolCap pool 0)"
-  "cap_master_arch_cap ( (arch_cap.PageTableCap ptr x)) =
-          (arch_cap.PageTableCap ptr None)"
-  "cap_master_arch_cap ( (arch_cap.PageDirectoryCap ptr y)) =
-          (arch_cap.PageDirectoryCap ptr None)"
-  "cap_master_arch_cap ( arch_cap.ASIDControlCap) =
-          arch_cap.ASIDControlCap"
+  "cap_master_arch_cap (ASIDPoolCap pool asid) = ASIDPoolCap pool 0"
+  "cap_master_arch_cap ASIDControlCap = ASIDControlCap"
+  "cap_master_arch_cap (IOPortCap first_port last_port) = IOPortCap 0 (-1)"
+  "cap_master_arch_cap (PageCap ref rghts maptype sz mapdata) = PageCap ref UNIV VMNoMap sz None"
+  "cap_master_arch_cap (PageTableCap ptr x) = PageTableCap ptr None"
+  "cap_master_arch_cap (PageDirectoryCap ptr x) = PageDirectoryCap ptr None"
+  "cap_master_arch_cap (PDPointerTableCap ptr x) = PDPointerTableCap ptr None"
+  "cap_master_arch_cap (PML4Cap ptr y) = PML4Cap ptr None"
   by (simp add: cap_master_arch_cap_def)+
 
 lemma aobj_ref_cases':
-  "aobj_ref acap = (case acap of arch_cap.ASIDControlCap \<Rightarrow> aobj_ref acap
+  "aobj_ref acap = (case acap of ASIDControlCap \<Rightarrow> aobj_ref acap
                                 | _ \<Rightarrow> aobj_ref acap)"
   by (simp split: arch_cap.split)
 
@@ -100,23 +101,26 @@ lemma aobj_ref_cases':
 lemma aobj_ref_cases:
   "aobj_ref acap = 
   (case acap of 
-    arch_cap.ASIDPoolCap w1 w2 \<Rightarrow> Some w1 
-  | arch_cap.ASIDControlCap \<Rightarrow> None
-  | arch_cap.PageCap w s sz opt \<Rightarrow> Some w
-  | arch_cap.PageTableCap w opt \<Rightarrow> Some w
-  | arch_cap.PageDirectoryCap w opt \<Rightarrow> Some w)"
+    ASIDPoolCap w1 w2 \<Rightarrow> Some w1 
+  | ASIDControlCap \<Rightarrow> None
+  | IOPortCap _ _ \<Rightarrow> None
+  | PageCap w s mt sz opt \<Rightarrow> Some w
+  | PageTableCap w opt \<Rightarrow> Some w
+  | PageDirectoryCap w opt \<Rightarrow> Some w
+  | PDPointerTableCap w opt \<Rightarrow> Some w
+  | PML4Cap w opt \<Rightarrow> Some w)"
   apply (subst aobj_ref_cases')
   apply (clarsimp cong: arch_cap.case_cong)
   done
 
 definition
   "cap_asid_base_arch cap \<equiv> case cap of 
-     (arch_cap.ASIDPoolCap _ asid) \<Rightarrow> Some asid
+     ASIDPoolCap _ asid \<Rightarrow> Some asid
   | _ \<Rightarrow> None"
 
 declare cap_asid_base_arch_def[abs_def, simp]
 
-definition
+definition cap_asid_base :: "cap \<Rightarrow> asid option" where
   "cap_asid_base cap \<equiv> arch_cap_fun_lift cap_asid_base_arch None cap"
 
 lemmas cap_asid_base_simps [simp] = 
@@ -152,7 +156,8 @@ lemma ups_of_heap_non_arch_upd:
   by (rule ext) (auto simp add: ups_of_heap_def non_arch_obj_def split: kernel_object.splits)
 
 definition
-  "is_simple_cap_arch cap \<equiv> \<not>is_pt_cap cap \<and> \<not> is_pd_cap cap"
+  "is_simple_cap_arch cap \<equiv> \<not>is_pt_cap cap \<and> \<not> is_pd_cap cap
+                          \<and> \<not> is_pdpt_cap cap \<and> \<not> is_pml4_cap cap"
 
 declare is_simple_cap_arch_def[simp]
 
@@ -170,8 +175,8 @@ lemma vs_cap_ref_to_table_cap_ref:
 
 
 lemma cap_master_cap_pg_cap: 
- "\<lbrakk>cap_master_cap cap = cap_master_cap capa\<rbrakk>
-  \<Longrightarrow> is_pg_cap cap = is_pg_cap capa"
+ "\<lbrakk>cap_master_cap cap = cap_master_cap cap'\<rbrakk>
+  \<Longrightarrow> is_pg_cap cap = is_pg_cap cap'"
   by (clarsimp simp:cap_master_cap_def is_cap_simps 
     split:cap.splits arch_cap.splits dest!:cap_master_cap_eqDs)
 
@@ -184,46 +189,51 @@ lemma master_arch_cap_cap_class:
   by (simp add: cap_master_arch_cap_def split: arch_cap.splits)
 
 lemma is_cap_free_index_update[simp]:
+  "is_pml4_cap (src_cap\<lparr>free_index := a\<rparr>) = is_pml4_cap src_cap"
+  "is_pdpt_cap (src_cap\<lparr>free_index := a\<rparr>) = is_pdpt_cap src_cap"
   "is_pd_cap (src_cap\<lparr>free_index := a\<rparr>) = is_pd_cap src_cap"
   "is_pt_cap (src_cap\<lparr>free_index := a\<rparr>) = is_pt_cap src_cap"
   by (simp add:is_cap_simps free_index_update_def split:cap.splits)+
 
 lemma masked_as_full_test_function_stuff[simp]:
-  "is_pd_cap (masked_as_full a cap ) = is_pd_cap a"
-  "is_pt_cap (masked_as_full a cap ) = is_pt_cap a"
-  "vs_cap_ref (masked_as_full a cap ) = vs_cap_ref a"
+  "is_pml4_cap (masked_as_full a cap) = is_pml4_cap a"
+  "is_pdpt_cap (masked_as_full a cap) = is_pdpt_cap a"
+  "is_pd_cap (masked_as_full a cap) = is_pd_cap a"
+  "is_pt_cap (masked_as_full a cap) = is_pt_cap a"
+  "vs_cap_ref (masked_as_full a cap) = vs_cap_ref a"
   by (auto simp:masked_as_full_def)
 
 lemma same_aobject_as_commute:
   "same_aobject_as x y \<Longrightarrow> same_aobject_as y x"
-  by (cases x; cases y; clarsimp)
+  by (cases x; cases y; clarsimp simp: same_aobject_as_def)
 
 lemmas wellformed_cap_simps = wellformed_cap_def
   [simplified wellformed_acap_def, split_simps cap.split arch_cap.split]
 
 lemma same_master_cap_same_types:
   "cap_master_cap cap = cap_master_cap cap' \<Longrightarrow>
-    (is_pt_cap cap = is_pt_cap cap') \<and> (is_pd_cap cap = is_pd_cap cap')"
+    (is_pt_cap cap = is_pt_cap cap') \<and> (is_pd_cap cap = is_pd_cap cap') \<and>
+    (is_pdpt_cap cap = is_pdpt_cap cap') \<and> (is_pml4_cap cap = is_pml4_cap cap')"
   by (clarsimp simp: cap_master_cap_def is_cap_simps 
                   split: cap.splits arch_cap.splits)
 
 lemma is_derived_cap_arch_asid_issues:
   "is_derived_arch cap cap' \<Longrightarrow>
     cap_master_cap cap = cap_master_cap cap'
-      \<Longrightarrow> ((is_pt_cap cap \<or> is_pd_cap cap) \<longrightarrow> cap_asid cap \<noteq> None)
+      \<Longrightarrow> (is_vspace_table_cap cap \<longrightarrow> cap_asid cap \<noteq> None)
              \<and> (is_pg_cap cap \<or> (vs_cap_ref cap = vs_cap_ref cap'))"
   apply (simp add: is_derived_arch_def)
-  by (auto simp: cap_master_cap_def is_cap_simps 
-                  cap_asid_def
-                  split: cap.splits arch_cap.splits option.splits)
+  by (auto simp: cap_master_cap_def is_cap_simps cap_asid_def
+          split: cap.splits arch_cap.splits option.splits)
 
-lemma is_pt_pd_Null[simp]:
-  "\<not> is_pt_cap cap.NullCap \<and> \<not> is_pd_cap cap.NullCap"
-  by (simp add: is_pt_cap_def is_pd_cap_def)
+lemma is_vspace_table_Null[simp]:
+  "\<not> is_pt_cap NullCap \<and> \<not> is_pd_cap NullCap \<and> \<not> is_pdpt_cap NullCap \<and> \<not> is_pml4_cap NullCap"
+  by (simp add: is_pt_cap_def is_pd_cap_def is_pdpt_cap_def is_pml4_cap_def)
 
 lemma unique_table_caps_upd_eqD: 
   "\<lbrakk>ms a = Some b; cap_asid b = cap_asid b'; obj_refs b = obj_refs b';
-    is_pd_cap b = is_pd_cap b'; is_pt_cap b = is_pt_cap b'\<rbrakk>
+    is_pd_cap b = is_pd_cap b'; is_pt_cap b = is_pt_cap b';
+    is_pdpt_cap b = is_pdpt_cap b'; is_pml4_cap b = is_pml4_cap b'\<rbrakk>
    \<Longrightarrow> unique_table_caps (ms (a \<mapsto> b')) = unique_table_caps (ms)"
   unfolding unique_table_caps_def
   apply (rule iffI)
@@ -245,12 +255,13 @@ lemma unique_table_caps_upd_eqD:
   apply (simp add: if_distrib split:if_splits)
   done
 
+(* FIXME: unused *)
 lemma set_untyped_cap_as_full_not_final_not_pg_cap:
-  "\<lbrace>\<lambda>s. (\<exists>a b. (a, b) \<noteq> dest \<and> \<not> is_pg_cap cap' 
+  "\<lbrace>\<lambda>s. (\<exists>a b. (a, b) \<noteq> dest \<and> \<not> is_pg_cap cap'
             \<and> cte_wp_at (\<lambda>cap. obj_irq_refs cap = obj_irq_refs cap' \<and> \<not> is_pg_cap cap) (a, b) s)
       \<and> cte_wp_at (op = src_cap) src s\<rbrace>
-  set_untyped_cap_as_full src_cap cap src 
-  \<lbrace>\<lambda>_ s.(\<exists>a b. (a, b) \<noteq> dest \<and> \<not> is_pg_cap cap' 
+  set_untyped_cap_as_full src_cap cap src
+  \<lbrace>\<lambda>_ s.(\<exists>a b. (a, b) \<noteq> dest \<and> \<not> is_pg_cap cap'
             \<and> cte_wp_at (\<lambda>cap. obj_irq_refs cap = obj_irq_refs cap' \<and> \<not> is_pg_cap cap) (a, b) s)\<rbrace>"
   apply (rule hoare_pre)
   apply (wp hoare_vcg_ex_lift)
