spec/abstract/X64/ArchCSpace_A.thy
@@ -25,43 +25,51 @@ text {* For some purposes capabilities to physical objects are treated
 differently to others. *}
 definition
   arch_is_physical :: "arch_cap \<Rightarrow> bool" where
-  "arch_is_physical cap \<equiv> case cap of ASIDControlCap \<Rightarrow> False | _ \<Rightarrow> True"
+  "arch_is_physical cap \<equiv> case cap of
+                            ASIDControlCap \<Rightarrow> False
+                          | IOPortCap _ _ \<Rightarrow> False
+                          | _ \<Rightarrow> True"
 
 text {* Check whether the second capability is to the same object or an object
 contained in the region of the first one. *}
 fun
   arch_same_region_as :: "arch_cap \<Rightarrow> arch_cap \<Rightarrow> bool"
 where
-  "arch_same_region_as (PageCap r R t s m) (PageCap r' R' t' s' m') =
+  "arch_same_region_as (PageCap r R t s m) c' =
+   (\<exists> r' R' t' s' m'. c' = PageCap r' R' t' s' m' \<and>
    (let
-     topA = r + (1 << pageBitsForSize s) - 1;
-     topB = r' + (1 << pageBitsForSize s') - 1
-   in r \<le> r' \<and> topA \<ge> topB \<and> r' \<le> topB)"
-| "arch_same_region_as (PageTableCap r _) c = (is_PageTableCap c \<and> aobj_ref c = Some r)"
-| "arch_same_region_as (PageDirectoryCap r _) c = (is_PageDirectoryCap c \<and> aobj_ref c = Some r)"
-| "arch_same_region_as (PDPointerTableCap r _) c = (is_PDPointerTableCap c \<and> aobj_ref c = Some r)"
-| "arch_same_region_as (PML4Cap r _) c = (is_PML4Cap c \<and> aobj_ref c = Some r)"
-| "arch_same_region_as ASIDControlCap c = (c = ASIDControlCap)"
-| "arch_same_region_as (ASIDPoolCap r _) c = (is_ASIDPoolCap c \<and> aobj_ref c = Some r)"
+      topA = r + (1 << pageBitsForSize s) - 1;
+      topB = r' + (1 << pageBitsForSize s') - 1
+    in r \<le> r' \<and> topA \<ge> topB \<and> r' \<le> topB))"
+| "arch_same_region_as (PageTableCap r _) c' = (\<exists>r' d'. c' = PageTableCap r' d' \<and> r = r')"
+| "arch_same_region_as (PageDirectoryCap r _) c' = (\<exists>r' d'. c' = PageDirectoryCap r' d' \<and> r = r')"
+| "arch_same_region_as (PDPointerTableCap r _) c' = (\<exists>r' d'. c' = PDPointerTableCap r' d' \<and> r = r')"
+| "arch_same_region_as (PML4Cap r _) c' = (\<exists>r' d'. c' = PML4Cap r' d' \<and> r = r')"
+| "arch_same_region_as ASIDControlCap c' = (c' = ASIDControlCap)"
+| "arch_same_region_as (ASIDPoolCap r _) c' = (\<exists>r' d'. c' = ASIDPoolCap r' d' \<and> r = r')"
 (* FIXME x64-vtd: *)
 (*
 | "arch_same_region_as (IOPageTableCap r _ _) c = (is_IOPageTableCap c \<and> aobj_ref c = Some r)"
 | "arch_same_region_as (IOSpaceCap d_id pci_d) c = (is_IOSpaceCap c \<and> cap_io_pci_device c = pci_d)"
-*)
   --"FIXME: should this also check domain id equality? C kernel does not"
-| "arch_same_region_as (IOPortCap frst lst) c = (is_IOPortCap c)"
-  --"FIXME: would an interval check make sense here?"
-| "arch_same_region_as _ _ = False"
+*)
+| "arch_same_region_as (IOPortCap frst lst) c' =
+   (\<exists>frst' lst'. c' = IOPortCap frst' lst' \<and> frst \<le> frst' \<and> lst' \<le> lst)"
 
 text {* Check whether two arch capabilities are to the same object. *}
 definition
   same_aobject_as :: "arch_cap \<Rightarrow> arch_cap \<Rightarrow> bool" where
  "same_aobject_as cp cp' \<equiv>
    (case (cp, cp') of
-      (PageCap ref _ _ pgsz _,PageCap ref' _ _ pgsz' _)
+      (PageCap ref _ _ pgsz _, PageCap ref' _ _ pgsz' _)
           \<Rightarrow> (ref, pgsz) = (ref', pgsz')
               \<and> ref \<le> ref + 2 ^ pageBitsForSize pgsz - 1
+    | (IOPortCap frst lst, IOPortCap frst' lst')
+          \<Rightarrow> (frst, lst) = (frst', lst')
     | _ \<Rightarrow> arch_same_region_as cp cp')"
+
+(* Proofs don't want to see this definition *)
+declare same_aobject_as_def[simp]
 
 text {* Only caps with sufficient rights can be recycled. *}
 definition
